completeness: Signature expansions. Countably many new nominals

Hybrid/Completeness/Lindenbaum/Expansion.lean
@@ -6,33 +6,283 @@ namespace Completeness
 open Completeness
 
 variable {α : Type u}
-variable [DecidableEq α]
+variable {β : Type v}
 
 /--
   TODO SECTION:
     Signature / Symbols extensions and embeddings.
     Properties preserved by embeddings.
 -/
-structure Symbols.morphism (S₁ : Symbols α) (S₂ : Symbols β) : Type u where
+structure Symbols.morphism (S₁ : Symbols α) (S₂ : Symbols β) : Type max (u+1) (v+1) where
   morph_sort : S₁.signature.S → S₂.signature.S
-  morph_op   : S₁.signature.Sig dom rng → S₂.signature.Sig (dom.map morph_sort) (morph_sort rng)
-  morph_N : S₁.signature.N st → S₂.signature.N (morph_sort st)
-  morph_prop : S₁.prop st → S₂.prop (morph_sort st)
-  morph_nom : S₁.nom st → S₂.nom (morph_sort st)
-  morph_svar : S₁.svar st → S₂.svar (morph_sort st)
-
-def Symbols.morphism.morph_premise {S₁ : Symbols α} {s : S₁.signature.S} (Γ : PremiseSet S₁ s) (m : Symbols.morphism S₁ S₂) : PremiseSet S₂ (m.morph_sort s) := sorry
-
-def Symbols.morphism.morph_axiom {S₁ : Symbols α} (Λ : AxiomSet S₁) (m : Symbols.morphism S₁ S₂) : AxiomSet S₂ := sorry
+  morph_op {dom rng} : S₁.signature.Sig dom rng → S₂.signature.Sig (dom.map morph_sort) (morph_sort rng)
+  morph_N    {st} : S₁.signature.N st → S₂.signature.N (morph_sort st)
+  morph_prop {st} : S₁.prop st → S₂.prop (morph_sort st)
+  morph_nom  {st} : S₁.nom st → S₂.nom (morph_sort st)
+  morph_svar {st} : S₁.svar st → S₂.svar (morph_sort st)
 
 structure Symbols.embedding (S₁ : Symbols α) (S₂ : Symbols β) where
-  m : Symbols.morphism S₁ S₂
-  -- m is injective
+  m : S₁.morphism S₂
+  sort_inj : m.morph_sort.Injective
+  op_inj   : ∀ dom rng, (@m.morph_op dom rng).Injective
+  N_inj    : ∀ st, (@m.morph_N st).Injective
+  prop_inj : ∀ st, (@m.morph_prop st).Injective
+  nom_inj  : ∀ st, (@m.morph_nom st).Injective
+  svar_inj : ∀ st, (@m.morph_svar st).Injective
 
-omit α in
-def Symbols.new_nominals (S₁ : Symbols α) : Σ S₂ : Symbols (ℕ ⊕ α), Symbols.embedding S₁ S₂ := sorry
+infix:50 "↪" => Symbols.embedding
 
-lemma SatLift {S₁ : Symbols α} {s : S₁.signature.S} {Λ : AxiomSet S₁} {S₂ : Symbols β} {Γ : PremiseSet S₁ s} {m : Symbols.embedding S₁ S₂} :
-  (m.m.morph_premise Γ).satisfiable (Models.Ax $ m.m.morph_axiom Λ) ↔ Γ.satisfiable (Models.Ax $ Λ) := sorry
+section Helpers
+
+  variable {S₁ : Symbols α}
+  variable {S₂ : Symbols β}
+  variable {s : S₁.signature.S}
+
+  def Symbols.morphism.morph_nominal (nom : S₁.nominal s) (m : S₁.morphism S₂) : S₂.nominal (m.morph_sort s) :=
+    match nom with
+    | .inl n => m.morph_N n
+    | .inr n => m.morph_nom n
+
+  def Symbols.morphism.morph_formula {sorts : List S₁.signature.S} (φ : FormL S₁ sorts) (m : S₁.morphism S₂) : FormL S₂ (sorts.map m.morph_sort) :=
+    match φ with
+    | .prop p   => .prop $ m.morph_prop p
+    | .nom  n   => .nom $ m.morph_nominal n
+    | .svar x   => .svar $ m.morph_svar x
+    | .or φ ψ   => .or (m.morph_formula φ) (m.morph_formula ψ)
+    | .neg φ    => .neg $ m.morph_formula φ
+    | @FormL.at _ _ _ s k φ   => ℋ@[[(m.morph_sort s)]] (m.morph_nominal k) (m.morph_formula φ)
+    | .bind x φ => .bind (m.morph_svar x) (m.morph_formula φ)
+    | .appl σ φ => .appl (m.morph_op σ) (m.morph_formula φ)
+    | .cons φ ψ => .cons (m.morph_formula φ) (m.morph_formula ψ)
+
+  def Symbols.morphism.morph_premise (Γ : PremiseSet S₁ s) (m : S₁.morphism S₂) : PremiseSet S₂ (m.morph_sort s) :=
+    { m.morph_formula φ | φ ∈ Γ }
+
+  abbrev Symbols.embedding.morph_formula (φ : Form S₁ s) (m : S₁ ↪ S₂) : Form S₂ (m.m.morph_sort s) :=
+    m.m.morph_formula φ
+
+  abbrev Symbols.embedding.morph_premise (Γ : PremiseSet S₁ s) (m : S₁ ↪ S₂) : PremiseSet S₂ (m.m.morph_sort s) :=
+    m.m.morph_premise Γ
+
+  section ClassicalRequired
+
+    open Classical
+
+    noncomputable def Symbols.morphism.morph_axiom (Λ : AxiomSet S₁) (m : S₁.morphism S₂) : AxiomSet S₂ :=
+      λ s => if h : ∃ s_inv, s = m.morph_sort s_inv then
+                { h.choose_spec ▸ m.morph_formula φ | φ ∈ Λ h.choose }
+             else { }
+
+    abbrev Symbols.embedding.morph_axiom (Λ : AxiomSet S₁) (m : S₁ ↪ S₂) : AxiomSet S₂ :=
+      m.m.morph_axiom Λ
+
+  end ClassicalRequired
+
+  notation:50 emb:lead "+" s:arg => Symbols.morphism.morph_sort (Symbols.embedding.m emb) s
+  notation:50 emb:lead "+" φ:arg => Symbols.embedding.morph_formula φ emb
+  notation:50 emb:lead "+" Γ:arg => Symbols.embedding.morph_premise Γ emb
+  notation:50 emb:lead "+" Λ:arg => Symbols.embedding.morph_axiom Λ emb
+
+end Helpers
+
+section Lemmas
+
+  variable {β : Type u}
+  variable {S₁ : Symbols α}
+  variable {s : S₁.signature.S}
+  variable {Λ : AxiomSet S₁}
+  variable {S₂ : Symbols β}
+  variable {m : S₁ ↪ S₂}
+
+  lemma SatLift {Γ : PremiseSet S₁ s} :
+    (m+ Γ).satisfiable (m+ Λ).Models ↔ Γ.satisfiable Λ.Models := by
+    apply Iff.intro
+    . intro ⟨M_plus, ⟨g_plus, ⟨w_plus, h⟩⟩⟩
+
+      admit
+    . intro ⟨M, ⟨g, ⟨w, h⟩⟩⟩
+      admit
+
+  lemma ProvableLift [DecidableEq α] [DecidableEq β] {φ : Form S₁ s} :
+    ⊢(m+ Λ, m+ s) (m+ φ) ↔ ⊢(Λ, s) φ := by
+
+      admit
+
+end Lemmas
+
+section NewNominals
+  /-
+    In this section, we (nonconstructively) define the extension of a signature with a countable set of new nominals,
+      and prove the new signature properly embeds the original one.
+
+    The main statement is `theorem Symbols.new_nominals`.
+  -/
+
+  abbrev Set.embed : Set α → Set (ℕ ⊕ α) := λ S => { Sum.inr e | e ∈ S }
+
+  abbrev Set.Elem.image {S : Set α} (e : S) : S.embed :=
+    ⟨Sum.inr e, by simp only [Set.mem_setOf_eq, Sum.inr.injEq, exists_eq_right, Subtype.coe_prop]⟩
+
+  noncomputable abbrev Set.Elem.preimage {S : Set α} (e : S.embed) : S :=
+    ⟨e.2.choose, e.2.choose_spec.1⟩
+
+  noncomputable abbrev List.preimage {S : Set α} (L : List S.embed): List S := L.map Set.Elem.preimage
+
+  lemma Set.Elem.preimage_injective {S : Set α} : (@Set.Elem.preimage α S).Injective := by
+    intro e1 e2 h
+    obtain ⟨e1, pf1⟩ := e1
+    obtain ⟨e2, pf2⟩ := e2
+    simp only [Set.mem_setOf_eq, Subtype.mk.injEq]
+    cases e1 with
+    | inl n =>
+      simp [Set.embed] at pf1
+    | inr a =>
+      cases e2 with
+      | inl n =>
+        simp [Set.embed] at pf2
+      | inr b =>
+        simp only [Sum.inr.injEq]
+        have a_choice := pf1.choose_spec.2
+        have b_choice := pf2.choose_spec.2
+        simp at a_choice b_choice h
+        rw [←a_choice, ←b_choice, h]
+
+  lemma Set.Elem.image_preimage_inv' {S : Set α} (e : S) : e.image.preimage = e := by
+    have := e.image.2.choose_spec.2
+    obtain ⟨e, pf⟩ := e
+    simp_all only [Subtype.mk.injEq, Sum.inr.injEq]
+
+  lemma Set.Elem.image_preimage_inv {S : Set α} : (@Set.Elem.preimage α S) ∘ Set.Elem.image = id := by
+    funext
+    apply Set.Elem.image_preimage_inv'
+
+  theorem Symbols.new_nominals (S₁ : Symbols α) : ∃ S₂ : Symbols (ℕ ⊕ α), Nonempty (S₁ ↪ S₂) :=
+    ⟨
+      {
+        signature := {
+          S := S₁.signature.S.embed
+          Sig := λ dom rng =>
+            (S₁.signature.Sig dom.preimage rng.preimage).embed,
+          N := λ st =>
+            (S₁.signature.N st.preimage).embed,
+          sortsCtbl := by
+            apply Countable.mk
+            have ⟨S₁_f, S₁_f_inj⟩ := S₁.signature.sortsCtbl.exists_injective_nat'
+            let f : S₁.signature.S.embed → ℕ := S₁_f ∘ Set.Elem.preimage
+            exists f
+            rw [Function.Injective.of_comp_iff]
+            . exact Set.Elem.preimage_injective
+            . exact S₁_f_inj,
+          opsCtbl := by
+            intro dom rng
+            apply Countable.mk
+            have ⟨S₁_f, S₁_f_inj⟩ := (S₁.signature.opsCtbl dom.preimage rng.preimage).exists_injective_nat'
+            let f : (S₁.signature.Sig dom.preimage rng.preimage).embed → ℕ := S₁_f ∘ Set.Elem.preimage
+            exists f
+            rw [Function.Injective.of_comp_iff]
+            . exact Set.Elem.preimage_injective
+            . exact S₁_f_inj,
+          nomCtbl := by
+            intro st
+            apply Countable.mk
+            have ⟨S₁_f, S₁_f_inj⟩ := (S₁.signature.nomCtbl st.preimage).exists_injective_nat'
+            let f : (S₁.signature.N st.preimage).embed → ℕ := S₁_f ∘ Set.Elem.preimage
+            exists f
+            rw [Function.Injective.of_comp_iff]
+            . exact Set.Elem.preimage_injective
+            . exact S₁_f_inj,
+          sNonEmpty := ⟨S₁.signature.sNonEmpty.default.image⟩
+        },
+        prop := λ st =>
+            (S₁.prop st.preimage).embed,
+        nom := λ st =>
+            (S₁.nom st.preimage).embed ∪ { Sum.inl n | n : ℕ },
+        svar := λ st =>
+            (S₁.svar st.preimage).embed,
+        propCtbl := by
+            intro st
+            apply Countable.mk
+            have ⟨S₁_f, S₁_f_inj⟩ := (S₁.propCtbl st.preimage).exists_injective_nat'
+            let f : (S₁.prop st.preimage).embed → ℕ := S₁_f ∘ Set.Elem.preimage
+            exists f
+            rw [Function.Injective.of_comp_iff]
+            . exact Set.Elem.preimage_injective
+            . exact S₁_f_inj,
+        nomCtbl := by
+            intro st
+            rw [Set.countable_union]
+            apply And.intro
+            . apply Countable.mk
+              have ⟨S₁_f, S₁_f_inj⟩ := (S₁.nomCtbl st.preimage).exists_injective_nat'
+              let f : (S₁.nom st.preimage).embed → ℕ := S₁_f ∘ Set.Elem.preimage
+              exists f
+              rw [Function.Injective.of_comp_iff]
+              . exact Set.Elem.preimage_injective
+              . exact S₁_f_inj
+            . rw [Set.countable_iff_exists_surjective]
+              . exists (λ n => ⟨.inl n, by simp⟩)
+                intro ⟨a, ⟨n, h⟩⟩
+                exists n
+                simp [h]
+              . exists .inl 0
+                simp,
+        svarCtbl := by
+            intro st
+            apply Countable.mk
+            have ⟨S₁_f, S₁_f_inj⟩ := (S₁.svarCtbl st.preimage).exists_injective_nat'
+            let f : (S₁.svar st.preimage).embed → ℕ := S₁_f ∘ Set.Elem.preimage
+            exists f
+            rw [Function.Injective.of_comp_iff]
+            . exact Set.Elem.preimage_injective
+            . exact S₁_f_inj,
+        propNonEmpty := λ s => ⟨(S₁.propNonEmpty s.preimage).default.image⟩
+      },
+      ⟨{
+        m := {
+          morph_sort := Set.Elem.image
+          morph_op := λ σ =>
+            ⟨Sum.inr σ,
+            by simp; rw [Set.Elem.image_preimage_inv, Set.Elem.image_preimage_inv']; simp⟩,
+          morph_N := λ j =>
+            ⟨Sum.inr j,
+            by simp; rw [Set.Elem.image_preimage_inv']; simp⟩,
+          morph_prop := λ p =>
+            ⟨Sum.inr p,
+            by simp; rw [Set.Elem.image_preimage_inv']; simp⟩,
+          morph_nom := λ j =>
+            ⟨Sum.inr j,
+            by simp; rw [Set.Elem.image_preimage_inv']; simp⟩,
+          morph_svar :=  λ x =>
+            ⟨Sum.inr x,
+            by simp; rw [Set.Elem.image_preimage_inv']; simp⟩,
+        },
+        sort_inj := by
+          simp
+          intro _ _
+          aesop,
+        op_inj := by
+          simp
+          intros _ _ _ _ _
+          aesop,
+        N_inj := by
+          simp
+          intros _ _ _
+          aesop,
+        prop_inj := by
+          simp
+          intros _ _ _
+          aesop,
+        nom_inj := by
+          simp
+          intros _ _ _
+          aesop,
+        svar_inj := by
+          simp
+          intros _ _ _
+          aesop
+      }⟩
+    ⟩
+
+end NewNominals
 
 end Completeness
